CookLevin/Complexity.lean
@@ -28,6 +28,7 @@ import Complexity.NP.SAT.CookLevin.Reductions.FrontLifting
 import Complexity.NP.SAT.CookLevin.Reductions.FrontProgram
 import Complexity.NP.SAT.CookLevin.Reductions.FrontWitness
 import Complexity.NP.SAT.CookLevin.Reductions.S1Map
+import Complexity.NP.SAT.CookLevin.Reductions.S1Program
 import Complexity.NP.SAT.CookLevin.Reductions.S1Witness
 import Complexity.NP.SAT.CookLevin.Reductions.S1Parse
 import Complexity.NP.SAT.CookLevin.Reductions.S1Cards
